Weidenbach_Book/IsaSAT_Initialisation.thy
@@ -2175,6 +2175,19 @@ proof -
     using pre ..
 qed
 
+definition (in -) ema_init where \<open>ema_init = 1 << 48\<close>
+
+lemma nat_of_uint64_ema_init_coeff: \<open>nat_of_uint64 ema_init = ema_init\<close>
+  unfolding ema_init_def
+  by transfer (auto simp: shiftl_nat_def)
+
+lemma (in -) ema_init_coeff_hnr[sepref_fr_rules]:
+  \<open>(uncurry0 (return ema_init), uncurry0 (RETURN ema_init)) \<in> unit_assn\<^sup>k \<rightarrow>\<^sub>a uint64_assn\<close>
+  by sepref_to_hoare 
+    (sep_auto simp: nat_of_uint64_ema_init_coeff uint64_nat_rel_def br_def)
+
+definition one_uint64 where [simp]: \<open>one_uint64 = 1\<close>
+
 text \<open>The value 160 is random (but larger than the default 16 for array lists).\<close>
 definition finalise_init_code :: \<open>twl_st_wl_heur_init \<Rightarrow> twl_st_wl_heur nres\<close> where
   \<open>finalise_init_code =
@@ -2182,8 +2195,8 @@ definition finalise_init_code :: \<open>twl_st_wl_heur_init \<Rightarrow> twl_st
        lbd, vdom). do {
      ASSERT(lst_As \<noteq> None \<and> fst_As \<noteq> None);
      let init_stats = (0::uint64, 0::uint64, 0::uint64, 0::uint64);
-     let fema = (0 :: uint64);
-     let sema = (0 :: uint64);
+     let fema = ema_init;
+     let sema = ema_init;
      let ccount = zero_uint32;
     RETURN (M', N', D', Q', W', ((ns, m, the fst_As, the lst_As, next_search), to_remove), \<phi>,
        clvls, cach, lbd, take1(replicate 160 (Pos zero_uint32_nat)), init_stats,
@@ -2274,6 +2287,8 @@ lemma (in -)empty_array_init_rll:
   apply (intro frefI nres_relI)
   apply  (auto simp: init_rll_def hr_comp_def clauses_ll_assn_def
     list_fmap_rel_def init_rll_list_def init_aa_def init_aa'_def)
+    apply (case_tac i)
+    apply auto
     apply (case_tac i)
     apply auto
   done
