Weidenbach_Book/IsaSAT_Restart.thy
@@ -1,5 +1,5 @@
 theory IsaSAT_Restart
-  imports Watched_Literals_Watch_List_Domain_Restart  IsaSAT_Setup
+  imports Watched_Literals_Watch_List_Domain_Restart IsaSAT_Setup IsaSAT_VMTF
 begin
 
 
@@ -22,8 +22,259 @@ text \<open>
        \<^text>\<open>conflictsRestarts > LOWER_BOUND_FOR_BLOCKING_RESTART && lbdQueue.isvalid() && trail.size() > R * trailQueue.getavg()\<close>
 \<close>
 
-context isasat_restart_bounded
+lemma unbounded_id: \<open>unbounded (id :: nat \<Rightarrow> nat)\<close>
+  by (auto simp: bounded_def) presburger
+
+locale isasat_restart_bounded' =
+  isasat_input_bounded
+
+context isasat_restart_bounded'
 begin
+text \<open>
+  We first fix the function that proves termination. We don't take the ``smallest'' function
+  possible (other possibilites that are growing slower include \<^term>\<open>\<lambda>(n::nat). n >> 50\<close>).
+\<close>
+sublocale isasat_restart_bounded id
+  by standard (rule unbounded_id)
+
+definition find_local_restart_target_level_int_inv where
+  \<open>find_local_restart_target_level_int_inv ns cs =
+     (\<lambda>(brk, i). i \<le> length cs \<and> length cs < uint32_max)\<close>
+
+definition find_local_restart_target_level_int :: \<open>trail_pol \<Rightarrow> vmtf_remove_int \<Rightarrow> nat nres\<close> where
+  \<open>find_local_restart_target_level_int =
+     (\<lambda>(M, xs, lvls, reasons, k, cs) ((ns, m, fst_As, lst_As, next_search), to_remove). do {
+     (brk, i) \<leftarrow> WHILE\<^sub>T\<^bsup>find_local_restart_target_level_int_inv ns cs\<^esup>
+        (\<lambda>(brk, i). \<not>brk \<and> i < length_u cs)
+        (\<lambda>(brk, i). do {
+           ASSERT(i < length cs);
+           let t = (cs  ! i);
+           ASSERT(t < length M);
+           ASSERT(M ! t \<in># \<L>\<^sub>a\<^sub>l\<^sub>l);
+           let L = atm_of (M ! t);
+           ASSERT(L < length ns);
+           let brk = stamp (ns ! L) < m;
+           RETURN (brk, if brk then i else i+one_uint32_nat)
+         })
+        (False, zero_uint32_nat);
+    RETURN i
+   })\<close>
+
+sepref_thm find_local_restart_target_level_code
+  is \<open>uncurry find_local_restart_target_level_int\<close>
+  :: \<open>trail_pol_assn\<^sup>k *\<^sub>a vmtf_remove_conc\<^sup>k \<rightarrow>\<^sub>a uint32_nat_assn\<close>
+  supply [[goals_limit=1]] length_rev[simp del]
+  unfolding find_local_restart_target_level_int_def find_local_restart_target_level_int_inv_def
+  by sepref
+
+definition (in isasat_input_ops) find_local_restart_target_level where
+  \<open>find_local_restart_target_level M _ = SPEC(\<lambda>i. i \<le> count_decided M)\<close>
+
+lemma find_local_restart_target_level_alt_def:
+  \<open>find_local_restart_target_level M vm = do {
+      (b, i) \<leftarrow> SPEC(\<lambda>(b::bool, i). i \<le> count_decided M);
+       RETURN i
+    }\<close>
+  unfolding find_local_restart_target_level_def by (auto simp: RES_RETURN_RES2 uncurry_def)
+
+lemma trail_pol_alt_def:
+  \<open>trail_pol = {((M', xs, lvls, reasons, k, cs), M). ((M', reasons), M) \<in> ann_lits_split_reasons \<and>
+    no_dup M \<and>
+    (\<forall>L \<in># \<L>\<^sub>a\<^sub>l\<^sub>l. nat_of_lit L < length xs \<and> xs ! (nat_of_lit L) = polarity M L) \<and>
+    (\<forall>L \<in># \<L>\<^sub>a\<^sub>l\<^sub>l. atm_of L < length lvls \<and> lvls ! (atm_of L) = get_level M L) \<and>
+    k = count_decided M \<and>
+    (\<forall>L\<in>set M. lit_of L \<in># \<L>\<^sub>a\<^sub>l\<^sub>l) \<and>
+    control_stack cs M \<and> literals_are_in_\<L>\<^sub>i\<^sub>n_trail M \<and>
+   length M < uint32_max \<and>
+   length M \<le> uint32_max div 2 + 1 \<and>
+   count_decided M < uint32_max \<and>
+   length M' = length M \<and>
+   M' = map lit_of (rev M)
+   }\<close>
+proof -
+  have [intro!]: \<open>length M < n \<Longrightarrow> count_decided M < n\<close> for M n
+    using length_filter_le[of is_decided M]
+    by (auto simp: literals_are_in_\<L>\<^sub>i\<^sub>n_trail_def uint_max_def count_decided_def
+        simp del: length_filter_le
+        dest: length_trail_uint_max_div2)
+  show ?thesis
+    unfolding trail_pol_def
+    by (auto simp: literals_are_in_\<L>\<^sub>i\<^sub>n_trail_def uint_max_def ann_lits_split_reasons_def
+        dest: length_trail_uint_max_div2)
+qed
+
+lemma find_local_restart_target_level_int_find_local_restart_target_level:
+   \<open>(uncurry find_local_restart_target_level_int, uncurry find_local_restart_target_level) \<in>
+     [\<lambda>(M, vm). vm \<in> vmtf M]\<^sub>f trail_pol \<times>\<^sub>r Id \<rightarrow> \<langle>nat_rel\<rangle>nres_rel\<close>
+  unfolding find_local_restart_target_level_int_def find_local_restart_target_level_alt_def
+    uncurry_def Let_def
+  apply (intro frefI nres_relI)
+  apply clarify
+  subgoal for a aa ab ac ad b ae af ag ah ba bb ai aj ak al am bc bd
+    apply (refine_rcg WHILEIT_rule[where R = \<open>measure (\<lambda>(brk, i). (If brk 0 1) + length b - i)\<close>]
+        assert.ASSERT_leI)
+    subgoal by auto
+    subgoal
+      unfolding find_local_restart_target_level_int_inv_def
+      by (auto simp: trail_pol_alt_def control_stack_length_count_dec)
+    subgoal by auto
+    subgoal by (auto simp: trail_pol_alt_def intro: control_stack_le_length_M)
+    subgoal by (auto simp: trail_pol_alt_def rev_map lits_of_def rev_nth
+          intro!: literals_are_in_\<L>\<^sub>i\<^sub>n_trail_in_lits_of_l)
+    subgoal by (auto simp: vmtf_def atms_of_def)
+    subgoal by (auto simp: find_local_restart_target_level_int_inv_def)
+    subgoal by (auto simp: trail_pol_alt_def control_stack_length_count_dec
+          find_local_restart_target_level_int_inv_def)
+    subgoal by auto
+    done
+  done
+
+definition (in isasat_input_ops) find_local_restart_target_level_st :: \<open>twl_st_wl_heur \<Rightarrow> nat nres\<close> where
+  \<open>find_local_restart_target_level_st S =
+     find_local_restart_target_level (get_trail_wl_heur S) (get_vmtf_heur S)\<close>
+
+lemma find_local_restart_target_level_st_alt_def:
+  \<open>find_local_restart_target_level_st = (\<lambda>(M, N, D, Q, W, vm, \<phi>, clvls, cach, lbd, stats).
+      find_local_restart_target_level M vm)\<close>
+  apply (intro ext)
+  apply (case_tac x)
+  by (auto simp: find_local_restart_target_level_st_def)
+
+definition (in isasat_input_ops) empty_Q :: \<open>twl_st_wl_heur \<Rightarrow> twl_st_wl_heur nres\<close> where
+  \<open>empty_Q = (\<lambda>(M, N, D, Q, W, vm, \<phi>, clvls, cach, lbd, stats). do{
+     RETURN (M, N, D, {#}, W, vm, \<phi>, clvls, cach, lbd, stats)
+  })\<close>
+
+
+definition (in isasat_input_ops) restart_abs_wl_heur_pre  :: \<open>twl_st_wl_heur \<Rightarrow> bool \<Rightarrow> bool\<close> where
+  \<open>restart_abs_wl_heur_pre S brk  \<longleftrightarrow> (\<exists>T. (S, T) \<in> twl_st_heur \<and> restart_abs_wl_D_pre T brk)\<close>
+
+text \<open>TODO when \<^term>\<open>lvl = count_decided M\<close>, we probably don't want to restart at all.\<close>
+definition (in isasat_input_ops) cdcl_twl_local_restart_wl_D_heur
+   :: \<open>twl_st_wl_heur \<Rightarrow> twl_st_wl_heur nres\<close>
+where
+  \<open>cdcl_twl_local_restart_wl_D_heur = (\<lambda>S. do {
+      ASSERT(restart_abs_wl_heur_pre S False);
+      lvl \<leftarrow> find_local_restart_target_level_st S;
+      if lvl = count_decided (get_trail_wl_heur S)
+      then RETURN S
+      else do {
+        S \<leftarrow> empty_Q S;
+        ASSERT(find_decomp_w_ns_pre ((get_trail_wl_heur S, lvl), get_vmtf_heur S));
+        find_decomp_wl_st_int lvl S
+      }
+   })\<close>
+
+named_theorems twl_st_heur
+
+lemma [twl_st_heur]:
+  assumes \<open>(S, T) \<in> twl_st_heur\<close>
+  shows \<open>get_trail_wl T = get_trail_wl_heur S\<close>
+  using assms by (cases S; cases T; auto simp: twl_st_heur_def; fail)
+
+
+lemma restart_abs_wl_D_pre_find_decomp_w_ns_pre:
+  assumes
+    pre: \<open>restart_abs_wl_D_pre T False\<close> and
+    ST: \<open>(S, T) \<in> twl_st_heur\<close> and
+    \<open>lvl < count_decided (get_trail_wl_heur S)\<close>
+  shows \<open>find_decomp_w_ns_pre ((get_trail_wl_heur S, lvl), get_vmtf_heur S)\<close>
+proof -
+  obtain x xa where
+    lits: \<open>literals_are_\<L>\<^sub>i\<^sub>n T\<close> and
+    Tx: \<open>(T, x) \<in> state_wl_l None\<close> and
+    \<open>partial_correct_watching T\<close> and
+    xxa: \<open>(x, xa) \<in> twl_st_l None\<close> and
+    struct: \<open>twl_struct_invs xa\<close> and
+    \<open>twl_list_invs x\<close> and
+    \<open>clauses_to_update_l x = {#}\<close> and
+    \<open>twl_stgy_invs xa\<close> and
+    \<open>get_conflict xa = None\<close>
+    using pre unfolding restart_abs_wl_D_pre_def restart_abs_wl_pre_def restart_abs_l_pre_def
+      restart_prog_pre_def
+    by blast
+  have \<open>literals_are_in_\<L>\<^sub>i\<^sub>n_trail (get_trail_wl_heur S)\<close>
+    using literals_are_\<L>\<^sub>i\<^sub>n_literals_are_\<L>\<^sub>i\<^sub>n_trail[OF Tx struct xxa lits] ST
+    by (auto simp add: twl_st_heur)
+  moreover have \<open> get_vmtf_heur S \<in> vmtf (get_trail_wl_heur S)\<close>
+    using ST by (auto simp add: twl_st_heur_def)
+  moreover have \<open>no_dup (get_trail_wl_heur S)\<close>
+    using struct ST Tx xxa unfolding twl_struct_invs_def cdcl\<^sub>W_restart_mset.cdcl\<^sub>W_all_struct_inv_def
+      cdcl\<^sub>W_restart_mset.cdcl\<^sub>W_M_level_inv_def by (auto simp: twl_st twl_st_l twl_st_heur)
+  ultimately show ?thesis
+    using assms unfolding find_decomp_w_ns_pre_def prod.case
+    by blast
+qed
+
+(* TODO Move *)
+lemma no_dup_appendD1:
+  \<open>no_dup (a @ b) \<Longrightarrow> no_dup a\<close>
+  by (auto simp: no_dup_def)
+(* End Move *)
+
+lemma cdcl_twl_local_restart_wl_D_spec_int:
+  \<open>cdcl_twl_local_restart_wl_D_spec (M, N, D, NE, UE, Q, W) \<ge> ( do {
+      ASSERT(restart_abs_wl_D_pre (M, N, D, NE, UE, Q, W) False);
+      i \<leftarrow> SPEC(\<lambda>_. True);
+      if i
+      then RETURN (M, N, D, NE, UE, Q, W)
+      else do {
+        (M, Q') \<leftarrow> SPEC(\<lambda>(M', Q'). (\<exists>K M2. (Decided K # M', M2) \<in> set (get_all_ann_decomposition M) \<and>
+              Q' = {#}) \<or> (M' = M \<and> Q' = Q));
+        RETURN (M, N, D, NE, UE, Q', W)
+     }
+   })\<close>
+proof -
+  have If_Res: \<open>(if i then (RETURN f) else (RES g)) = (RES (if i then {f} else g))\<close> for i f g
+    by auto
+  have H: \<open>g = g' \<Longrightarrow> (f \<bind> g) = (f \<bind> g')\<close> for f :: \<open>_ nres\<close> and g g' by auto
+  show ?thesis
+    unfolding cdcl_twl_local_restart_wl_D_spec_def prod.case RES_RETURN_RES2 If_Res
+    by refine_vcg
+      (auto simp: If_Res RES_RETURN_RES2 RES_RES_RETURN_RES uncurry_def
+        image_iff split:if_splits)
+qed
+
+lemma cdcl_twl_local_restart_wl_D_heur_cdcl_twl_local_restart_wl_D_spec:
+  \<open>(cdcl_twl_local_restart_wl_D_heur, cdcl_twl_local_restart_wl_D_spec) \<in>
+    twl_st_heur \<rightarrow>\<^sub>f \<langle>twl_st_heur\<rangle>nres_rel\<close>
+proof -
+  have [dest]: \<open>av = None\<close> \<open>out_learned a av am \<Longrightarrow> out_learned x1 av am\<close>
+    if \<open>restart_abs_wl_D_pre (a, au, av, aw, ax, ay, bd) False\<close>
+    for a au av aw ax ay bd x1 am
+    using that
+    unfolding restart_abs_wl_D_pre_def restart_abs_wl_pre_def restart_abs_l_pre_def
+      restart_prog_pre_def
+    by (auto simp: twl_st_l_def state_wl_l_def out_learned_def)
+  have [dest]: \<open>find_decomp_w_ns_pre ((a, lvl), (ae, af, ag, ah, b), ba) \<Longrightarrow>
+       (Decided K # x1, M2) \<in> set (get_all_ann_decomposition a) \<Longrightarrow>
+        no_dup x1\<close>
+    for a lvl ae ab ag ah b ba x1 M2 af K
+    unfolding find_decomp_w_ns_pre_def prod.case
+    by (auto dest!: distinct_get_all_ann_decomposition_no_dup no_dup_appendD1)
+  have [refine0]:
+    \<open>SPEC (\<lambda>i. i \<le> count_decided a) \<le> \<Down> {(i, b). b = (i = count_decided a) \<and>
+          i \<le> count_decided a} (SPEC (\<lambda>_. True))\<close> for a
+    by (auto intro: RES_refine)
+  show ?thesis
+    unfolding cdcl_twl_local_restart_wl_D_heur_def
+      find_decomp_wl_st_int_def find_local_restart_target_level_def
+      find_decomp_w_ns_def empty_Q_def find_local_restart_target_level_st_def
+    apply (intro frefI nres_relI)
+    apply clarify
+    apply (rule ref_two_step)
+     prefer 2
+     apply (rule cdcl_twl_local_restart_wl_D_spec_int)
+    unfolding bind_to_let_conv Let_def RES_RETURN_RES2
+    apply (refine_vcg )
+    subgoal unfolding restart_abs_wl_heur_pre_def by blast
+    subgoal by auto
+    subgoal
+      by (force dest: restart_abs_wl_D_pre_find_decomp_w_ns_pre)
+    subgoal
+      by (rule RES_refine)  (force simp: twl_st_heur_def intro!: )
+    done
+qed
 
 definition remove_all_annot_true_clause_imp_wl_D_heur_inv
   :: \<open>twl_st_wl_heur \<Rightarrow> nat list \<Rightarrow> nat \<times> twl_st_wl_heur \<Rightarrow> bool\<close>
@@ -84,7 +335,7 @@ definition restart_required_heur :: "twl_st_wl_heur \<Rightarrow> nat \<Rightarr
     RETURN (
        ((get_slow_ema_heur S * 5) >> 2) > get_fast_ema_heur S \<and>
         get_conflict_count_heur S > minimum_number_between_restarts \<and>
-        size (get_clauses_wl_heur S) > f n)\<close>
+        size (get_clauses_wl_heur S) > n)\<close>
 
 
 end
